In your initial post, address the following:

# Compare proof by contradiction and proof by contrapositive
A proof by contradiction assumes the theorem is false and tries to show inconsistency; meanwhile, a proof by contrapositive assumes the conclusion is false and proves the negation of the hypothesis.  Determining which to use, if either can be applied, should be based on which one provides a more useful assumption to work with.  Both can be used to show inconsistency in a given assumption.  Below is an example of a proof by contradiction:

# Provide an example of one or the other.
Assumption:
For every pair of positive real numbers, a and b,
<math xmlns="http://www.w3.org/1998/Math/MathML">
  <msqrt>
    <mi>a</mi>
  </msqrt>
  <mo>+</mo>
  <msqrt>
    <mi>b</mi>
  </msqrt>
  <mo>&#x2260;<!-- â‰  --></mo>
  <msqrt>
    <mo stretchy="false">(</mo>
    <mi>a</mi>
    <mo>+</mo>
    <mi>b</mi>
    <mo stretchy="false">)</mo>
  </msqrt>
</math>

<br><br>
Proof: Suppose there are two real numbers, a and b, such that a > 0, b > 0 and <math xmlns="http://www.w3.org/1998/Math/MathML">
  <msqrt>
    <mi>a</mi>
  </msqrt>
  <mo>+</mo>
  <msqrt>
    <mi>b</mi>
  </msqrt>
</math>
 = <math xmlns="http://www.w3.org/1998/Math/MathML">
  <msqrt>
    <mo stretchy="false">(</mo>
    <mi>a</mi>
    <mo>+</mo>
    <mi>b</mi>
    <mo stretchy="false">)</mo>
  </msqrt>
</math>

<br><br>
<math xmlns="http://www.w3.org/1998/Math/MathML">
  <mo stretchy="false">(</mo>
  <msqrt>
    <mi>a</mi>
  </msqrt>
  <mo>+</mo>
  <msqrt>
    <mi>b</mi>
  </msqrt>
  <msup>
    <mo stretchy="false">)</mo>
    <mn>2</mn>
  </msup>
  <mo>=</mo>
  <mo stretchy="false">(</mo>
  <msqrt>
    <mo stretchy="false">(</mo>
    <mi>a</mi>
    <mo>+</mo>
    <mi>b</mi>
    <mo stretchy="false">)</mo>
  </msqrt>
  <msup>
    <mo stretchy="false">)</mo>
    <mn>2</mn>
  </msup>
</math>

<br>
<math xmlns="http://www.w3.org/1998/Math/MathML">
  <mo stretchy="false">(</mo>
  <msqrt>
    <mi>a</mi>
  </msqrt>
  <msup>
    <mo stretchy="false">)</mo>
    <mn>2</mn>
  </msup>
  <mo>+</mo>
  <mn>2</mn>
  <msqrt>
    <mo stretchy="false">(</mo>
    <mi>a</mi>
    <mi>b</mi>
    <mo stretchy="false">)</mo>
  </msqrt>
  <mo>+</mo>
  <mo stretchy="false">(</mo>
  <msqrt>
    <mi>b</mi>
  </msqrt>
  <msup>
    <mo stretchy="false">)</mo>
    <mn>2</mn>
  </msup>
  <mo>=</mo>
  <mi>a</mi>
  <mo>+</mo>
  <mi>b</mi>
</math>

<br>
<math xmlns="http://www.w3.org/1998/Math/MathML">
  <mi>a</mi>
  <mo>+</mo>
  <mn>2</mn>
  <msqrt>
    <mo stretchy="false">(</mo>
    <mi>a</mi>
    <mi>b</mi>
    <mo stretchy="false">)</mo>
  </msqrt>
  <mo>+</mo>
  <mi>b</mi>
  <mo>=</mo>
  <mi>a</mi>
  <mo>+</mo>
  <mi>b</mi>
</math>

<br>
<math xmlns="http://www.w3.org/1998/Math/MathML">
  <mn>2</mn>
  <msqrt>
    <mo stretchy="false">(</mo>
    <mi>a</mi>
    <mi>b</mi>
    <mo stretchy="false">)</mo>
  </msqrt>
  <mo>=</mo>
  <mn>0</mn>
</math>

<br>
<math xmlns="http://www.w3.org/1998/Math/MathML">
  <mi>a</mi>
  <mi>b</mi>
  <mo>=</mo>
  <mn>0</mn>
</math>

Since ab = 0, then a = 0 or b = 0.This fact is inconsistent with the assumption that  a > 0 and b > 0. <div id="36" class="animation-object animation-box-object ember-view" style="top: 480px; left: 510px; opacity: 1; background-color: rgb(51, 51, 51); height: 3px; width: 3px; border-color: rgb(51, 51, 51); transform: rotateZ(0deg);"></div>

Note: To use LaTeX within the discussion, use the equation editor. For your LaTeX to show up inline, enclose it withBackslash, open parenthesis, ellipses, backslash, close parenthesis. If you would like to enter a LaTeX item in your Brightspace discussion post, look on the menu bar for your post between the subject and text areas, click on the Sigma icon, and choose LaTeX equation. If you cannot see the Sigma icon, click on the three dots at the extreme right of the menu bar (to the right of Font Family, Font Size, etc.) to show all of the icons.